Main.lean
@@ -32,18 +32,18 @@ lf {
           meta    [startup, shutdown]
         }
         body {
-          let w ← getState s
-          let x ← getInput i
-          let y ← getInput n₂.o
+          let w ← getState  s
+          let x ← getInput  i
+          let y ← getInput  n₂.o
           let z ← getAction ActionSource.a
-          let p ← getParam p
+          let p ← getParam  p
           let t ← getTag
           let l ← getLogicalTime
           let q ← getPhysicalTime
-          setState s w
-          setOutput o true
+          setOutput o    true
           setOutput n₁.i (-1)
-          schedule a (.of 10 .s) "hello"
+          setState  s    w
+          schedule  a    (.of 10 .s) "hello"
         }
       }
     ]
@@ -60,17 +60,37 @@ lf {
     reactions   []
 } 
 
-macro val:term " -[" i:term "]→ " p:term : term => `(ReactionM.ReactionSatisfiesM $val $i $p)
+open Lean in
+macro input:term " -[" rcn:ident "]→ " prop:term : term =>
+  `($(mkIdent `ReactionSatisfiesM) $input $(mkIdentFrom rcn <| `LF ++ rcn.getId ++ `body) $prop)
 
--- TODO: Have the reactions array contain the bodies, not the reaction.
+-- TODO: 0. Generalize this to use `SatisfiesM.bind`.
+--       1. Turn this into an elab that reads p from the goal state.
+--       2. Find a way to "output" a goal over ReactionSatisfiesM instead of SatisfiesM.
+--       3. Remove the explicit goal tag, since there's only a single goal.
+open Lean in
+macro "resolve_bind" p:term:max proof:term : tactic => 
+  `(tactic| (
+      apply SatisfiesM.bind_pre
+      simp [$(mkIdent `Input.noop):ident]
+      refine SatisfiesM.imp ?next (p := $p) (by
+        intro output h
+        apply SatisfiesM.pure
+        revert h
+        exact $proof
+      )
+    )
+  )
+
 open LF ReactionM
-example : Main.reactions[0].val.body -[input]→ 
-  (·.fst.state .s = ReactionM.Input.state input Main.State.s) := by
-  let output := do
-    setOutput .o true
-    setOutput .n₁.i (-1 : Int)
-    schedule  .a (.of 10 .s) sorry
-  let x := output input
-  exists (return ⟨x, by sorry⟩)
-  sorry
-
+example : input -[Main.Reaction0]→ (·.fst.state .s = input.state .s) := by
+  simp [Main.Reaction0]
+  iterate 7 resolve_bind (·.fst.state .s = input.state .s) (by rw [Output.merge_state, ·])
+  apply SatisfiesM.bind (p := (·.fst.state .s = input.state .s))
+  · resolve_bind (fun _ => True) (by simp)
+    exact SatisfiesM.trivial
+  · simp [Input.noop]
+    intro output h
+    iterate 4 resolve_bind (·.fst.state .s = input.state .s) (by rw [Output.merge_state, ·])
+    apply SatisfiesM.pure
+    simp [h]
